Started ch2

Definitions/Semantics.v
@@ -1,20 +1,57 @@
 From Definitions Require Export Combinators.
 
-Inductive exec : combinator -> combinator -> Prop :=
-| ExecB : forall x y z, exec (B @ x @ y @ z) (x @ (y @ z))
-| ExecC : forall x y z, exec (C @ x @ y @ z) (x @ z @ y)
-| ExecK : forall x y,   exec (K @ x @ y) x
-| ExecW : forall x y,   exec (W @ x @ y) (x @ y @ y)
-| ExecNull: forall x,   exec x x.
-(* | ExecL : forall x y z, exec x y -> exec (x @ z) (y @ z)
-| ExecR : forall x y z, exec x y -> exec (z @ x) (z @ y). *)
+Create HintDb hclt.
+Ltac hauto := eauto with hclt.
 
-Notation "a ~> b" := (exec a b) (at level 55, left associativity).
+Reserved Notation "a ~> b" (at level 20).
+Inductive sstep : combinator -> combinator -> Prop :=
+| ExecB : forall x y z, (B @ x @ y @ z) ~> (x @ (y @ z))
+| ExecC : forall x y z, (C @ x @ y @ z) ~> (x @ z @ y)
+| ExecK : forall x y,   (K @ x @ y) ~> x
+| ExecW : forall x y,   (W @ x @ y) ~> (x @ y @ y)
+| ExecAppL : forall x x' y, x ~> x' -> (x @ y) ~> (x' @ y)
+| ExecAppR : forall x y y', y ~> y' -> (x @ y) ~> (x @ y')
+    where "a ~> b" := (sstep a b).
+
+Hint Constructors sstep : hclt.
 
 Inductive Q : combinator -> combinator -> Prop :=
 | Def2 : forall x y, x = y -> Q x y
 | Qlr : forall x y, x ~> y -> Q x y
 | Qrl : forall x y, y ~> x -> Q x y
-| Qmid1 : forall x y x' y', x ~> x' -> y ~> y' -> Q x' y' -> Q x y
-| Qmid2 : forall x y x' y', x' ~> x -> y' ~> y -> Q x' y' -> Q x y
-| RuleQ2 : forall x y w, Q x y -> Q (w @ x) (w @ y).
+| Qstepl : forall x x' y, x ~> x' -> Q x' y -> Q x y
+| Qstepr : forall x y y', y ~> y' -> Q x y' -> Q x y
+| Q_trans : forall x y z, Q x y -> Q y z -> Q x z. 
+
+Hint Constructors Q : hclt.
+
+(* Definition 3 *)
+Definition _I := W @ K.
+
+(* Remark *)
+Definition _S : combinator :=
+    B @ (B @ (B @ W) @ C) @ (B @ B).
+
+Theorem Q_app_l : forall x y w,
+    Q x y -> Q (w @ x) (w @ y).
+Proof with hauto.
+    intros. induction H... subst...
+Qed.
+
+Theorem RuleB : forall x y z,
+    Q (B @ x @ y @ z) (x @ (y @ z)).
+Proof. hauto. Qed.
+
+Theorem RuleC : forall x y z,
+    Q (C @ x @ y @ z) (x @ z @ y).
+Proof. hauto. Qed.
+
+Theorem RuleW : forall x y,
+    Q (W @ x @ y) (x @ y @ y).
+Proof. hauto. Qed.
+
+Theorem RuleK : forall x y,
+    Q (K @ x @ y) x.
+Proof. hauto. Qed.
+
+Hint Resolve Q_app_l RuleB RuleC RuleW RuleK : hclt.
