Proofs/Part1/Ch1D.v
@@ -1,50 +1,103 @@
 From Definitions Require Export Combinators Semantics.
 
+(* Theorem 1 *)
 Theorem Q_refl:
     forall x, Q x x.
-Proof.
-    intros. apply Def2.
-    reflexivity.
-Qed.
+Proof. hauto. Qed.
 
+(* Theorem 2 *)
 Theorem Q_sym:
     forall x y, Q x y -> Q y x.
-Proof.
-    intros. induction H; subst.
-    apply Def2. reflexivity.
-    apply Qrl. assumption.
-    apply Qlr. assumption.
-    apply (Qmid1 y x y' x'); try assumption.
-    apply (Qmid2 y x y' x'); try assumption.
-    apply RuleQ2. assumption.
+Proof with hauto. 
+    intros; induction H...
+    Unshelve. exact B.
 Qed.
 
-(* Lemma test:
-    forall x y z,
-    y ~> x -> Q y z -> Q x z.
-Proof.
-    intros. induction H0; subst.
-    apply Qrl. assumption.
-    apply (Qmid2 x y x0 x0); try assumption. apply Q_refl.
-    apply (Qmid2 x y x0 y). 
-        assumption. apply ExecNull. apply Qrl. assumption.
-     *)
-
+(* Theorem 3 *)
 Theorem Q_trans:
     forall x y z, Q x y -> Q y z -> Q x z.
+Proof. hauto. Qed.
+
+(* Theorem 4 *)
+Theorem Q_app_r :
+    forall x y z,
+    Q x y -> Q (x @ z) (y @ z).
+Proof with hauto.
+    intros; induction H...
+    subst...
+Qed.
+
+(* Theorem 6 *)
+Require Export Coq.Classes.RelationClasses.
+Require Export Coq.Setoids.Setoid.
+
+Instance Q_equiv : Equivalence Q.
 Proof.
-    intros. induction H; subst.
-    assumption.
-    apply (Qmid1 x z y z). 
-        assumption. apply ExecNull. assumption.
-    apply (Qmid2 x z y z).
-        assumption. apply ExecNull. assumption.
-    apply (Qmid1 x z x' z).
-        assumption. apply ExecNull. apply IHQ.
-        apply (Qmid2 y' z y z). assumption. apply ExecNull. assumption.
-    apply (Qmid2 x z x' z).
-        assumption. apply ExecNull. apply IHQ.
-        apply (Qmid1 y' z y z). assumption. apply ExecNull. assumption.
-    induction H; subst.
-        assumption.
-Admitted.
+  constructor.
+    unfold Reflexive. apply Q_refl.
+    unfold Symmetric. apply Q_sym. 
+    unfold Transitive. apply Q_trans.
+Qed.
+
+Add Parametric Relation : combinator Q
+  reflexivity proved by Q_refl
+  symmetry proved by Q_sym
+  transitivity proved by Q_trans
+  as Q_setoid.
+
+(* Theorem 7 *)
+Require Import List.
+Export ListNotations.
+Fixpoint app_comb_list (l : list combinator) : option combinator :=
+    match l with
+    | [] => None
+    | h :: t =>
+        match app_comb_list t with
+        | None => Some h
+        | Some a => Some (a @ h)
+        end
+    end.
+
+Lemma app_comb_list_cons_inv :
+    forall h t1 t2 A B,
+    Some A = app_comb_list (h :: t1) ->
+    Some B = app_comb_list (h :: t2) ->
+    t1 = t2 ->
+    A = B.
+Proof.
+    intros. subst. rewrite <- H in H0.
+    now inversion H0.
+Qed.
+
+Theorem list_comb_app_inv :
+    forall (Xl Dl : list combinator)
+           (X D default : combinator)
+           (i : nat),
+    Some X = app_comb_list Xl ->
+    Some D = app_comb_list Dl ->
+    length Xl = length Dl ->
+    i < length Xl ->
+    nth i Xl default = nth i Dl default ->
+    X = D.
+Abort.
+
+(* Theorem 9 *)
+Theorem id_x : forall x,
+    Q (_I @ x) x.
+Proof. hauto. Qed.
+
+Corollary Schonfinkel_KSB :
+    Q B (_S @ (K @ _S) @ K).
+Abort.
+
+Corollary Schonfinkel_KSC :
+    Q C (_S @ (B @ B @ _S) @ (K @ K)).
+Abort.
+
+Corollary Schonfinkel_KSW :
+    Q W (_S @ _S @ (_S @ K)).
+Abort.
+
+Corollary Schonfinkel_KSI :
+    Q _I (_S @ K @ K).
+Abort.
