Proofs/Part1/Ch2B.v
@@ -1,0 +1,32 @@
+From Proofs Require Import Ch1D.
+
+(* Section 1 : The B Sequence *)
+Fixpoint B_seq (n : nat) : combinator :=
+    match n with
+    | 0 => _I
+    | 1 => B
+    | S n' => B @ B @ B_seq n'
+    end.
+
+Lemma B_seq_Sn : forall n,
+    1 <= n ->
+    B_seq (S n) = B @ B @ B_seq n.
+Proof. 
+    intros. simpl. destruct n. inversion H.
+    destruct n; simpl; reflexivity.
+Qed.
+
+(* Theorem 1 *)
+Theorem B_Sn_xyz__Bn_xyz :
+    forall x y z n,
+    Q (B_seq (S n) @ x @ y @ z) (B_seq n @ x @ (y @ z)).
+Proof.
+    intros. destruct n.
+    - hauto.
+    - rewrite B_seq_Sn.
+        etransitivity.
+            apply Qlr. hauto.
+        etransitivity.
+            apply Qlr. hauto.
+        hauto. apply le_n_S, PeanoNat.Nat.le_0_l.
+Qed.
